LambdaS5/coq/LjsStore.v
@@ -16,11 +16,7 @@ Definition add_object st obj : (store * value) :=
   let ptr := fresh st in (st \(fresh st := obj), value_object ptr).
 
 Definition add_closure c recid args body : value :=
-  let si := match recid with 
-    | Some i => expr_fv (expr_lambda args body) \-- i
-    | None => expr_fv (expr_lambda args body) 
-    end in
-  value_closure (closure_intro (to_list (c \| si)) recid args body)
+  value_closure (closure_intro (to_list c) recid args body)
 .
 
 (* Adds function arguments to the lexical environment *)
